kill all sorries for konigs, wip on others

Matroid/Graph/Matching/Defs.lean
@@ -20,6 +20,7 @@ structure IsMatching (G : Graph α β) (M : Set β) : Prop where
 @[mk_iff]
 structure IsMaxMatching (G : Graph α β) (M : Set β) : Prop extends G.IsMatching M where
   max : ∀ M', G.IsMatching M' → M'.encard ≤ M.encard
+attribute [grind .] IsMatching.subset IsMatching.disjoint IsMaxMatching.max
 
 noncomputable def matchingNumber (G : Graph α β) : ℕ∞ :=
   sSup {n | ∃ M, G.IsMatching M ∧ n = M.encard}
@@ -28,6 +29,40 @@ scoped notation "ν(" G ")" => matchingNumber G
 
 def IsMatchable (G : Graph α β) (S : Set α) : Prop := ∃ M, G.IsMatching M ∧ V(G, M) = S
 
+def matchingNumberSet (G : Graph α β) : Set ℕ∞ :=
+  {n | ∃ M, G.IsMatching M ∧ n = M.encard}
+
+@[simp, grind =]
+lemma matchingNumberSet_eq : G.matchingNumberSet = {n | ∃ M, G.IsMatching M ∧ n = M.encard} := rfl
+
+@[simp, grind .]
+lemma IsMatching.encard_mem_matchingNumberSet (hM : G.IsMatching M) :
+    M.encard ∈ G.matchingNumberSet :=
+  ⟨M, hM, rfl⟩
+
+lemma IsMatching.encard_le (hM : G.IsMatching M) : M.encard ≤ ν(G) := by
+  unfold matchingNumber
+  refine le_sSup ?_
+  refine ⟨M, hM, rfl⟩
+
+lemma le_matchingNumber_of_mem_matchingNumberSet {n} (hn : n ∈ G.matchingNumberSet) : n ≤ ν(G) := by
+  obtain ⟨M, hM, rfl⟩ := hn
+  exact hM.encard_le
+
+lemma IsMaxMatching.encard (h : G.IsMaxMatching M) : M.encard = ν(G) := by
+  unfold matchingNumber
+  symm
+  refine IsGreatest.csSup_eq ?_
+  refine ⟨h.encard_mem_matchingNumberSet, ?_⟩
+  simp [upperBounds]
+  grind only [max]
+
+lemma IsMatching.isMaxMatching_of_encard_eq (hM : G.IsMatching M) (h : M.encard = ν(G)) :
+    G.IsMaxMatching M where
+  toIsMatching := hM
+  max M' hM' := by
+    rw [h]
+    exact hM'.encard_le
 
 lemma IsMatching.subsingleton_inc (h : G.IsMatching M) (v : α) : (M ∩ E(G, v)).Subsingleton := by
   intro e he f hf
@@ -49,29 +84,516 @@ lemma IsMatching.maxDegree_le_one [G.Loopless] (h : G.IsMatching M) : (G ↾ M).
   rw [eDegree_eq_encard_inc]
   exact this v
 
+-- I just realized the next 4ish lemmas are duplicates from `Matching/Def.lean`
+@[simp, grind .]
+lemma IsMatching.incEdges_subsingleton (hM : G.IsMatching M) (x : α) :
+    E(G ↾ M, x).Subsingleton := by
+  rw [incEdges_edgeRestrict]
+  intro e he f hf
+  by_contra! hcon
+  have disj := hM.disjoint he.2 hf.2 hcon
+  rw [Set.disjoint_left] at disj
+  have hxe : x ∈ V(G, e) := by grind
+  have hxf : x ∈ V(G, f) := by grind
+  exact disj hxe hxf
+
+@[simp, grind .]
+lemma IsMatching.incEdges_encard_le_one (hM : G.IsMatching M) (x : α) :
+    E(G ↾ M, x).encard ≤ 1 := by
+  rw [Set.encard_le_one_iff_subsingleton]
+  exact hM.incEdges_subsingleton x
+
+@[simp, grind .]
+lemma IsMatching.eDegree_le_one [G.Loopless] (hM : G.IsMatching M) (x : α) :
+    (G ↾ M).eDegree x ≤ 1 := by
+  rw [eDegree_eq_encard_inc]
+  exact hM.incEdges_encard_le_one x
+
+@[simp, grind .]
+lemma IsMatching.maxDegreeLE_one [G.Loopless] (hM : G.IsMatching M) : (G ↾ M).MaxDegreeLE 1 :=
+  fun x ↦ hM.eDegree_le_one x
+
+@[simp, grind .]
+lemma isMatching_empty : G.IsMatching ∅ := by
+  constructor <;> simp
+
+@[simp, grind .]
+lemma isMatching_singleton (he : e ∈ E(G)) : G.IsMatching {e} := by
+  constructor <;> [simpa ; simp]
+
+
 lemma IsMatching.of_le (hle : G ≤ H) (h : G.IsMatching M) : H.IsMatching M where
   subset := h.subset.trans (edgeSet_mono hle)
   disjoint e f heM hfM hne := by
-    -- Consider `disjoint_iff_forall_notMem` and`inc_eq_of_le`
-    sorry
+    unfold endSet
+    -- TODO: how to repeat a tactic exactly n times?
+    repeat rw [← inc_eq_of_le hle (h.subset ‹_›)]
+    exact h.disjoint heM hfM hne
 
-lemma IsMatching.encard_le (hM : G.IsMatching M) : M.encard ≤ ν(G) := by
-  sorry
+@[simp, grind .]
+lemma IsMatching.anti_left (hM : G.IsMatching M) (hle : H ≤ G) (hMH : M ⊆ E(H)) :
+    H.IsMatching M := by
+  refine ⟨hMH, ?_⟩
+  rintro e f heM hfM hne
+  refine disjoint_of_subset ?_ ?_ (hM.disjoint heM hfM hne)
+  all_goals exact endSet_mono hle _
 
-lemma IsMaxMatching.encard (h : G.IsMaxMatching M) : M.encard = ν(G) := by
-  sorry
+@[simp, grind .]
+lemma IsMatching.anti_right (hM : G.IsMatching M) (h : M' ⊆ M) : G.IsMatching M' := by
+  refine ⟨have := hM.subset; by grind, ?_⟩
+  intro e f heM' hfM' hne
+  exact hM.disjoint (h heM') (h hfM') hne
 
-lemma IsMatching.isMaxMatching_of_encard_eq (hM : G.IsMatching M) (h : M.encard = ν(G)) :
-    G.IsMaxMatching M where
-  toIsMatching := hM
-  max M' hM' := by
-    sorry
+/-- The restriction of a matching to a subgraph remains a matching. -/
+@[simp, grind .]
+lemma IsMatching.anti_left' (hM : G.IsMatching M) (hle : H ≤ G) :
+    H.IsMatching (E(H) ∩ M) := by
+  refine IsMatching.anti_left ?_ hle ?_
+  · exact hM.anti_right (by grind)
+  grind
 
-lemma IsMatching.isMaxMatching_of_vertex_subset (hM : G.IsMatching M) (hsu : V(G) ⊆ V(G, M)) :
-    G.IsMaxMatching M where
-  toIsMatching := hM
-  max M' hM' := by
-    sorry
+lemma isMatching_iff_edgeRestrict_isMatching :
+    G.IsMatching M ↔ (G ↾ M).IsMatching M := by
+  refine ⟨?_, ?_⟩
+  · intro hM
+    refine hM.anti_left edgeRestrict_le ?_
+    simp only [edgeRestrict_edgeSet, subset_inter_iff, subset_refl, and_true]
+    grind only [hM.subset]
+  intro hM
+  refine hM.of_le edgeRestrict_le
+
+lemma isMaxMatching_iff_maximalFor : G.IsMaxMatching M ↔ MaximalFor G.IsMatching Set.encard M :=
+  ⟨fun h => ⟨h.toIsMatching, fun T hT _ ↦ h.2 T hT⟩,
+    fun h => ⟨h.1, fun T hT ↦ (le_total T.encard M.encard).elim id <| h.2 hT⟩⟩
+
+lemma matchingNumber_mono (hle : G ≤ H) : ν(G) ≤ ν(H) := by
+  -- any matching of G can be lifted to a matching of H
+  conv => lhs; unfold matchingNumber
+  rw [sSup_le_iff]
+  rintro _ ⟨M, hM, rfl⟩
+  exact hM.of_le hle |>.encard_le
+
+-- If every vertex has at most 1 incident edge, then it must be a matching.
+lemma isMatching_of_encard_incEdges_le_one
+    (M : Set β)
+    (hM_subset : M ⊆ E(G))
+    (h : ∀ x ∈ V(G), E(G ↾ M, x).encard ≤ 1) :
+    G.IsMatching M where
+  subset := hM_subset
+  disjoint e f he hf hne := by
+    by_contra! hcon
+    rw [not_disjoint_iff_nonempty_inter] at hcon
+    obtain ⟨x, hxe, hxf⟩ := hcon
+    simp at hxe hxf
+    have hxP : x ∈ G.vertexSet := hxe.vertex_mem
+    simp only [incEdges_edgeRestrict, Set.encard_le_one_iff_subsingleton] at h
+    specialize h _ hxP ⟨hxe, he⟩ ⟨hxf, hf⟩
+    contradiction
+
+lemma isMatching_of_eDegree_le_one
+    (M : Set β)
+    (hM_subset : M ⊆ E(G))
+    (h : ∀ x ∈ V(G), (G ↾ M).eDegree x ≤ 1) :
+    G.IsMatching M where
+  subset := hM_subset
+  disjoint e f he hf hne := by
+    by_contra! hcon
+    rw [not_disjoint_iff_nonempty_inter] at hcon
+    obtain ⟨x, hxe, hxf⟩ := hcon
+    simp at hxe hxf
+    have hxP : x ∈ G.vertexSet := hxe.vertex_mem
+    replace h : ∀ x ∈ V(G), E(G ↾ M, x).encard ≤ 1 := by
+      intro x hx
+      grw [encard_setOf_inc_le_eDegree (G ↾ M) x]
+      exact h _ hx
+    simp only [incEdges_edgeRestrict, Set.encard_le_one_iff_subsingleton] at h
+    specialize h _ hxP ⟨hxe, he⟩ ⟨hxf, hf⟩
+    contradiction
+
+/-! ### Cover -/
+
+structure IsCover (G : Graph α β) (S : Set α) : Prop where
+  subset : S ⊆ V(G)
+  cover : E(G) ⊆ E(G, S)
+
+
+structure IsMinCover (G : Graph α β) (S : Set α) : Prop extends IsCover G S where
+  min : ∀ T, IsCover G T → S.encard ≤ T.encard
+
+noncomputable def coverNumber (G : Graph α β) : ℕ∞ :=
+  sInf {n | ∃ S, G.IsCover S ∧ n = S.encard}
+
+scoped notation "τ(" G ")" => coverNumber G
+
+def coverNumberSet (G : Graph α β) : Set ℕ∞ :=
+  {n | ∃ S, G.IsCover S ∧ n = S.encard}
+
+@[simp]
+lemma coverNumberSet_eq : G.coverNumberSet = {n | ∃ S, G.IsCover S ∧ n = S.encard} := rfl
+
+
+lemma IsCover.mem_or_mem_of_isLink (h : G.IsCover S) (he : G.IsLink e u v) : u ∈ S ∨ v ∈ S := by
+  have cover := h.cover
+  have e_mem : e ∈ E(G, S) := h.cover he.edge_mem
+  rw [mem_setIncEdges_iff] at e_mem
+  obtain ⟨x, hxS, hx⟩ := e_mem
+  have := hx.eq_or_eq_of_isLink he
+  grind
+
+lemma IsCover.le_encard (h : G.IsCover S) : τ(G) ≤ S.encard := by
+  unfold coverNumber
+  grind [sInf_le]
+
+lemma IsMinCover.encard (h : G.IsMinCover S) : S.encard = τ(G) := by
+  unfold coverNumber
+  refine le_antisymm ?_ h.le_encard
+  have := h.min
+  grind [le_sInf]
+
+lemma coverNumber_le_of_mem_coverNumberSet {n} (hn : n ∈ G.coverNumberSet) : τ(G) ≤ n := by
+  obtain ⟨S, hS, rfl⟩ := hn
+  exact hS.le_encard
+
+-- TODO: rename; unless we decide to drop the subset condition, then this becomes obsolete
+lemma IsCover.encard_le_vertexSet_encard (h : G.IsCover S) : S.encard ≤ V(G).encard := by
+  exact encard_le_encard h.subset
+
+lemma isMinCover_iff_minimalFor : G.IsMinCover S ↔ MinimalFor G.IsCover Set.encard S :=
+  ⟨fun h => ⟨h.toIsCover, fun T hT _ ↦ h.min T hT⟩,
+    fun h => ⟨h.1, fun T hT ↦ (le_total T.encard S.encard).elim (h.2 hT) id⟩⟩
+
+lemma IsCover.of_vertexDelete (h : (G - X).IsCover S) : G.IsCover ((V(G) ∩ X) ∪ S) where
+  subset := by
+    have := h.subset
+    simp at this
+    tauto_set
+  cover e he := by
+    rw [edge_mem_iff_exists_isLink] at he
+    obtain ⟨x, y, hexy⟩ := he
+    simp
+    wlog hx : x ∈ X ∨ x ∈ S with aux
+    · specialize aux h e y x hexy.symm
+      apply aux; clear aux
+      simp at hx
+      obtain (hy|hy) := em (y ∈ X)
+        <;> [left ; right]
+      · assumption
+      replace hexy : (G - X).IsLink e x y := by
+        refine hexy.of_le_of_mem vertexDelete_le ?_
+        -- TODO: add grind tags for these simps; in general whenever the pattern
+        -- `simp; grind` shows up, add grind tags to those simp lemmas
+        simp only [vertexDelete_edgeSet, mem_setOf_eq]; grind
+      grind [h.mem_or_mem_of_isLink hexy]
+    refine ⟨x, ?_, hexy.inc_left⟩
+    have : x ∈ V(G) := hexy.left_mem
+    grind
+
+
+lemma IsCover.isMinCover_of_encard_eq (hS : G.IsCover S) (h : S.encard = τ(G)) :
+    G.IsMinCover S where
+  toIsCover := hS
+  min T hT := by
+    grind [coverNumber, sInf_le]
+
+/-- There exists a trivial cover (the entire vertex set). -/
+lemma isCover_vertexSet (G : Graph α β) : G.IsCover V(G) where
+  subset := by rfl
+  cover e he := by
+    simpa only [setIncEdges_vertexSet]
+
+-- Might be useful to have it in `Exists` form
+lemma exists_isCover (G : Graph α β) : ∃ S, G.IsCover S := ⟨V(G), G.isCover_vertexSet⟩
+
+lemma vertexSet_encard_mem_coverNumberSet : V(G).encard ∈ G.coverNumberSet := by
+  simp
+  refine ⟨V(G), G.isCover_vertexSet, rfl⟩
+
+lemma coverNumberSet_nonempty : G.coverNumberSet.Nonempty := by
+  refine ⟨V(G).encard, vertexSet_encard_mem_coverNumberSet⟩
+
+lemma coverNumber_le_vertexSet_encard (G : Graph α β) : τ(G) ≤ V(G).encard := by
+  simp only [coverNumber]
+  refine sInf_le_of_le G.vertexSet_encard_mem_coverNumberSet (le_refl _)
+
+-- lemma exists_isMinCover_of_finite [G.Finite] : ∃ S, G.IsMinCover S := by
+--   have hle := G.coverNumber_le_vertexSet_encard
+--   have finite_encard : V(G).encard ≠ ⊤ := by
+--     have := G.vertexSet_finite
+--     exact encard_ne_top_iff.mpr this
+--   have solver : τ(G) ∈ G.coverNumberSet :=
+--     ENat.sInf_mem coverNumberSet_nonempty
+--   simp at solver
+--   obtain ⟨S, hS, hS_min⟩ := solver
+--   refine ⟨S, hS.isMinCover_of_encard_eq hS_min.symm⟩
+
+-- kinda wacky that this always exists...
+lemma exists_isMinCover (G : Graph α β) : ∃ S, G.IsMinCover S := by
+  have : τ(G) ∈ G.coverNumberSet := csInf_mem coverNumberSet_nonempty
+  simp at this
+  obtain ⟨S, hS, hS_min⟩ := this
+  refine ⟨S, hS.isMinCover_of_encard_eq hS_min.symm⟩
+
+lemma IsCover.intersect_endSet_nonempty (hS : G.IsCover S) (he : e ∈ E(G)) :
+    Nonempty ↑(S ∩ V(G, e)) := by
+  have ⟨x, y, hxy⟩ := exists_isLink_of_mem_edgeSet he
+  obtain (h|h) := hS.mem_or_mem_of_isLink hxy
+    <;> [refine ⟨x, ?_⟩ ; refine ⟨y, ?_⟩]
+    <;> tauto_set
+
+noncomputable def IsMatching.mapToCover (hM : G.IsMatching M) (hS : G.IsCover S) : M → S := by
+  -- we should be able to arbitrarily choose either vertex for any e ∈ M
+  intro ⟨e, he⟩
+  have heE : e ∈ E(G) := hM.subset he
+  -- take ends, cap with S?
+  have nonempty := hS.intersect_endSet_nonempty heE
+  obtain ⟨x, hx⟩ := Classical.choice nonempty
+  refine ⟨x, hx.1⟩
+
+-- set_option pp.proofs true in
+lemma IsMatching.mapToCover_inj (hM : G.IsMatching M) (hS : G.IsCover S) :
+    Function.Injective (hM.mapToCover hS) := by
+  intro ⟨e, he⟩ ⟨f, hf⟩ heq
+  simp only [Subtype.mk.injEq]
+  by_contra! hcon
+  unfold mapToCover at heq
+  simp at heq
+  -- TODO: this still feels suboptimal.
+  generalize_proofs ex ey at heq
+  -- this leaves `heq : ↑(Classical.choice ex) = ↑(Classical.choice ey)`
+  -- directly trying to destruct ex/ey with `obtain` messes things up
+  -- (it effectively undoes the `generalize_proofs`)
+  set x := Classical.choice ex
+  set y := Classical.choice ey
+  obtain ⟨x, hx⟩ := x
+  obtain ⟨y, hy⟩ := y
+  simp only at heq
+  have disj := hM.disjoint he hf hcon
+  refine disj.notMem_of_mem_left (a := x) hx.2 ?_
+  rw [heq]
+  exact hy.2
+
+-- set_option pp.proofs true in
+lemma IsMatching.mapToCover_inc (hM : G.IsMatching M) (hS : G.IsCover S) (he : e ∈ M) :
+    G.Inc e (hM.mapToCover hS ⟨e, he⟩) := by
+  simp only [mapToCover]
+  set x := (Classical.choice (IsCover.intersect_endSet_nonempty hS (hM.subset he)))
+  have hxE : ↑x ∈ V(G, e) := x.2.2
+  rwa [← mem_endSet_iff]
+
+lemma matchingNumber_le_coverNumber : ν(G) ≤ τ(G) := by
+  simp only [matchingNumber, coverNumber]
+  simp only [le_sInf_iff, sSup_le_iff]
+  rintro t ⟨C, hS, rfl⟩ n ⟨M, hM, rfl⟩
+  have solver := (hM.mapToCover_inj hS).encard_range
+  simp only [ENat.card_coe_set_eq, range] at solver
+  refine le_trans solver ?_
+  rw [show C.encard = (univ : Set ↑C).encard by simp]
+  refine encard_le_encard (by grind)
+
+lemma exists_isMaxMatching' (G : Graph α β) (hν : ν(G) ≠ ⊤) : ∃ M, G.IsMaxMatching M := by
+  have : ν(G) ∈ G.matchingNumberSet := by
+    have injOn : InjOn ENat.toNat G.matchingNumberSet := by
+      intro i hi j hj heq
+      have hi_le : i ≤ ν(G) := le_matchingNumber_of_mem_matchingNumberSet hi
+      have hj_le : j ≤ ν(G) := le_matchingNumber_of_mem_matchingNumberSet hj
+      enat_to_nat!
+      simp at heq
+      assumption
+    have im_eq : ENat.toNat '' G.matchingNumberSet ⊆ {i | i ≤ ν(G).toNat} := by
+      intro i hi
+      obtain ⟨n, hn, rfl⟩ := hi
+      obtain ⟨M, hM, rfl⟩ := hn
+      exact ENat.toNat_le_toNat hM.encard_le hν
+    have finite : G.matchingNumberSet.Finite := by
+      refine Set.Finite.of_finite_image ?_ injOn
+      refine Set.Finite.subset (finite_le_nat ν(G).toNat) im_eq
+    have : G.matchingNumberSet.Nonempty :=
+      ⟨0, ∅, isMatching_empty, encard_empty.symm⟩
+    exact this.csSup_mem finite
+  obtain ⟨M, hM, hM_eq⟩ := this
+  refine ⟨M, hM.isMaxMatching_of_encard_eq hM_eq.symm⟩
+
+lemma exists_isMaxMatching (G : Graph α β) [G.Finite] : ∃ M, G.IsMaxMatching M := by
+  refine G.exists_isMaxMatching' ?_
+  have := G.matchingNumber_le_coverNumber
+  have τ_finite : τ(G) < ⊤ := by
+        have : V(G).encard < ⊤ := encard_lt_top_iff.mpr ‹G.Finite›.vertexSet_finite
+        have := G.coverNumber_le_vertexSet_encard
+        enat_to_nat!
+  enat_to_nat!
+
+lemma IsMatching.encard_le_isCover_encard (hM : G.IsMatching M) (hS : G.IsCover S) :
+    M.encard ≤ S.encard := by
+  grw [hM.encard_le, ← hS.le_encard]
+  exact matchingNumber_le_coverNumber
+
+lemma IsMatching.mapToCover_range_eq_of_encard_eq [G.Finite]
+    (hS : G.IsCover S) (hM : G.IsMatching M) (h : S.encard = M.encard) :
+    range (hM.mapToCover hS) = S := by
+  have S_finite : S.Finite :=
+    Set.Finite.subset vertexSet_finite hS.subset
+  have M_finite : M.Finite :=
+    Set.Finite.subset edgeSet_finite hM.subset
+  have subset : Subtype.val '' range (hM.mapToCover hS) ⊆ S := by
+    simp only [image_subset_iff, Subtype.coe_preimage_self, subset_univ]
+    -- TODO: pain point, switching between encard and ncard
+    -- (need ncard because `Set.subset_iff_eq_of_ncard_le` has no encard equivalent)
+  have : (Subtype.val '' range (hM.mapToCover hS) |>.ncard) = M.ncard := by
+    simp only [ncard_image_of_injective _ Subtype.val_injective,
+      ncard_range_of_injective (hM.mapToCover_inj hS), Nat.card_coe_set_eq]
+  rwa [← subset_iff_eq_of_ncard_le ?_ S_finite]
+  simp only [← S_finite.cast_ncard_eq, ← M_finite.cast_ncard_eq, Nat.cast_inj] at h
+  rw [this, h]
+
+-- TODO: rename
+lemma IsCover.subgraph_cover (hS : H.IsCover S) (hle : G ≤ H) : G.IsCover (S ∩ V(G)) where
+  subset := by tauto_set
+  cover := by
+    intro e he
+    simp
+    have heH := (edgeSet_mono hle) he
+    rw [edge_mem_iff_exists_isLink] at he
+    obtain ⟨x, y, hexy⟩ := he
+    obtain h := hS.mem_or_mem_of_isLink (hexy.of_le hle)
+    wlog hxS : x ∈ S with aux
+    · specialize aux hS hle heH y x hexy.symm h.symm (by grind)
+      assumption
+    refine ⟨x, ⟨hxS, hexy.left_mem⟩, hexy.inc_left⟩
+
+lemma coverNumber_mono (hle : G ≤ H) : τ(G) ≤ τ(H) := by
+  have ⟨S_G, hS_G⟩ := G.exists_isMinCover
+  have ⟨S_H, hS_H⟩ := H.exists_isMinCover
+  have subcover := hS_H.subgraph_cover hle
+  have := hS_G.min _ subcover
+  grw [← hS_G.encard, this, ← hS_H.encard]
+  grind [encard_le_encard]
+
+-- You can take unions of matchings/covers across strongly disjoint graphs
+lemma IsCover.union {H₁ H₂ : Graph α β} {S₁ S₂ : Set α}
+    (hS₁ : H₁.IsCover S₁) (hS₂ : H₂.IsCover S₂) (hdisj : H₁.StronglyDisjoint H₂) :
+    (H₁ ∪ H₂).IsCover (S₁ ∪ S₂) where
+  subset := by grind [union_vertexSet, hS₁.subset, hS₂.subset]
+  cover := by
+    intro e
+    simp [hdisj.compatible.union_inc_iff]
+    rintro (he|he)
+    · apply exists_isLink_of_mem_edgeSet at he
+      obtain ⟨x, y, hexy⟩ := he
+      obtain (h|h) := hS₁.mem_or_mem_of_isLink hexy
+        <;> [use x; use y]
+        <;> refine ⟨Or.inl ‹_›, Or.inl ?_⟩
+        <;> [exact hexy.inc_left ; exact hexy.inc_right]
+    -- not sure how to golf this better
+    apply exists_isLink_of_mem_edgeSet at he
+    obtain ⟨x, y, hexy⟩ := he
+    obtain (h|h) := hS₂.mem_or_mem_of_isLink hexy
+      <;> [use x; use y]
+      <;> refine ⟨Or.inr ‹_›, Or.inr ?_⟩
+      <;> [exact hexy.inc_left ; exact hexy.inc_right]
+
+lemma IsMinCover.union {T : Set α}
+    (hS : G.IsMinCover S) (hT : H.IsMinCover T) (hdisj : G.StronglyDisjoint H) :
+    (G ∪ H).IsMinCover (S ∪ T) := by
+  refine ⟨hS.toIsCover.union hT.toIsCover hdisj, ?_⟩
+  intro A hA
+  have hAG : G.IsCover (A ∩ V(G)) :=
+    hA.subgraph_cover (G.left_le_union H)
+  have hAH : H.IsCover (A ∩ V(H)) := by
+    have : H ≤ G ∪ H := by grind only [hdisj.compatible.union_comm, Graph.left_le_union]
+    exact hA.subgraph_cover this
+  have ST_disj : Disjoint S T := by grind [hS.subset, hT.subset, hdisj.vertex]
+  rw [encard_union_eq ST_disj]
+  have : A = (A ∩ V(G)) ∪ (A ∩ V(H)) := by
+    have : V(G ∪ H) = V(G) ∪ V(H) := by exact union_vertexSet G H
+    grind [hA.subset]
+  rw [this,
+    encard_union_eq (show Disjoint (A ∩ V(G)) (A ∩ V(H)) by grind [hdisj.vertex])];
+    clear this
+  have hle1 := hAG.le_encard
+  have hle2 := hAH.le_encard
+  rw [hS.encard, hT.encard]
+  exact add_le_add hle1 hle2
+
+lemma IsMatching.union
+    {H₁ H₂ : Graph α β} {M₁ M₂ : Set β}
+    (hM₁ : H₁.IsMatching M₁)
+    (hM₂ : H₂.IsMatching M₂)
+    (hdisj : StronglyDisjoint H₁ H₂) :
+    (H₁ ∪ H₂).IsMatching (M₁ ∪ M₂) where
+  -- TODO: grind tags
+  subset := by grind [union_edgeSet, hM₁.subset, hM₂.subset]
+  disjoint e f he hf hne := by
+    have all_left {M : Set β} {H K : Graph α β}
+        (hM : H.IsMatching M) (hdisj : H.StronglyDisjoint K) :
+        ∀ ⦃e⦄, e ∈ M → V(H ∪ K, e) = V(H, e) := by
+      intro e he
+      ext x
+      simp only [endSet, mem_setOf_eq, hdisj.compatible.union_inc_iff]
+      refine ⟨?_, by grind⟩
+      rintro (_|h) <;> [assumption ; exfalso]
+      replace he : e ∈ E(H) := hM.subset he
+      grind [h.edge_mem, hdisj.edge]
+    have all_right : ∀ ⦃e⦄, e ∈ M₂ → V(H₁ ∪ H₂, e) = V(H₂, e) := by
+      have := all_left hM₂ hdisj.symm
+      simpa only [hdisj.compatible.union_comm]
+    specialize all_left hM₁ hdisj
+    match he, hf with
+    | Or.inl he, Or.inl hf
+    | Or.inr he, Or.inr hf =>
+      simp only [all_left, all_right, he, hf]
+      grind only [= disjoint_left, hM₁.disjoint, hM₂.disjoint]
+    | Or.inl he, Or.inr hf
+    | Or.inr he, Or.inl hf =>
+      simp only [all_left, all_right, he, hf]
+      grind only [hdisj.vertex, = disjoint_left, = mem_endSet_iff, → Inc.vertex_mem]
+
+lemma IsMaxMatching.union {N : Set β}
+    (hM : G.IsMaxMatching M) (hN : H.IsMaxMatching N) (hdisj : G.StronglyDisjoint H) :
+    (G ∪ H).IsMaxMatching (M ∪ N) := by
+  refine ⟨hM.toIsMatching.union hN.toIsMatching hdisj, ?_⟩
+  intro F hF
+  have hFG : G.IsMatching (E(G) ∩ F) := hF.anti_left' (G.left_le_union H)
+  have hFH : H.IsMatching (E(H) ∩ F) :=
+    hF.anti_left' <| by grind only [hdisj.compatible.union_comm, Graph.left_le_union]
+  rw [encard_union_eq (show Disjoint M N by grind [hM.subset, hN.subset, hdisj.edge]),
+    show F = (E(G) ∩ F) ∪ (E(H) ∩ F) by grind [hF.subset, union_edgeSet],
+    encard_union_eq (show Disjoint (E(G) ∩ F) (E(H) ∩ F) by grind [hdisj.edge]),
+    hM.encard, hN.encard]
+  have hle1 := hFG.encard_le
+  have hle2 := hFH.encard_le
+  exact add_le_add hle1 hle2
+
+@[simp, grind =]
+lemma coverNumber_union (hdisj : G.StronglyDisjoint H) : τ(G ∪ H) = τ(G) + τ(H) := by
+  obtain ⟨S, hS⟩ := G.exists_isMinCover
+  obtain ⟨T, hT⟩ := H.exists_isMinCover
+  have ST_minCover := hS.union hT hdisj
+  rw [← hS.encard, ← hT.encard, ← ST_minCover.encard]
+  refine encard_union_eq ?_
+  grind  [hdisj.vertex, hS.subset, hT.subset]
+
+@[simp, grind =]
+lemma matchingNumber_union (hdisj : G.StronglyDisjoint H) : ν(G ∪ H) = ν(G) + ν(H) := by
+  obtain (hinf|hfinite) := em' (ν(G) ≠ ⊤ ∧ ν(H) ≠ ⊤)
+  · wlog hν : (ν(G) = ⊤) with aux
+    · specialize aux hdisj.symm (by grind) (by grind)
+      rw [hdisj.compatible.union_comm, aux, add_comm]
+    simp [hν]
+    rw [matchingNumber, sSup_eq_top] at hν ⊢
+    intro b hb
+    obtain ⟨n, hn, hbn⟩ := hν b hb
+    obtain ⟨M, hM, rfl⟩ := hn
+    refine ⟨M.encard, ?_, hbn⟩
+    refine ⟨M, hM.of_le (G.left_le_union H), rfl⟩
+  obtain ⟨M, hM⟩ := G.exists_isMaxMatching' hfinite.1
+  obtain ⟨N, hN⟩ := H.exists_isMaxMatching' hfinite.2
+  have MN_maxMatching := hM.union hN hdisj
+  rw [← hM.encard, ← hN.encard, ← MN_maxMatching.encard]
+  refine encard_union_eq <| by grind [hdisj.edge, hM.subset, hN.subset]
+
+
+
+/-! ### restrict₂ (lemmas needed for Tutte-Berge?) -/
 
 def IsMatching.restrict₂ (hM : G.IsMatching M) (hM' : G.IsMatching M') : Graph α β :=
   G ↾ (M ∆ M') |>.loopRemove
@@ -84,12 +606,12 @@ lemma IsMatching.symmDiff_maxDegree_le_two (hM : G.IsMatching M) (hM' : G.IsMatc
     (hM.restrict₂ hM').MaxDegreeLE 2 := by
   sorry
 
-lemma IsMatching.disjoint_inter_of_isCycleGraph_symmDiff (hM : G.IsMatching M)
+lemma IsMatching.disjoint_inter_of_isCycle_symmDiff (hM : G.IsMatching M)
     (hM' : G.IsMatching M') (hC : C.IsCycle) (hCG : C ≤ hM.restrict₂ hM') :
     Disjoint (E(C) ∩ M) (E(C) ∩ M') := by
   sorry
 
-lemma IsMatching.inter_encard_eq_of_isCycleGraph_isCompOf_symmDiff (hM : G.IsMatching M)
+lemma IsMatching.inter_encard_eq_of_isCycle_isCompOf_symmDiff (hM : G.IsMatching M)
     (hM' : G.IsMatching M') (hC : C.IsCycle) (hCG : C.IsCompOf (hM.restrict₂ hM')) :
     (E(C) ∩ M).encard = (E(C) ∩ M').encard := by
   sorry
@@ -100,38 +622,46 @@ lemma IsMatching.inter_encard_eq_of_isCycleGraph_isCompOf_symmDiff (hM : G.IsMat
 --     ∃ G' : Graph α β, G'.IsCompOf (hM.restrict₂ hM') ∧ G'.IsPathGraph := by
 --   contrapose! hcd
 --   have hmax := hM.symmDiff_maxDegree_le_two hM'
---   have hcd' : ∀ (G' : Graph α β), G'.IsCompOf (hM.restrict₂ hM') → G'.IsCycleGraph :=
---     fun G' hG' ↦ hG'.isPathGraph_or_isCycleGraph_of_maxDegreeLE hmax |>.resolve_left
+--   have hcd' : ∀ (G' : Graph α β), G'.IsCompOf (hM.restrict₂ hM') → G'.IsCycle :=
+--     fun G' hG' ↦ hG'.isPathGraph_or_isCycle_of_maxDegreeLE hmax |>.resolve_left
 --     <| hcd G' hG'
 --   clear hcd hmax
 --   sorry -- component partition
 
-lemma isMaxMatching_iff_maximalFor : G.IsMaxMatching M ↔ MaximalFor G.IsMatching Set.encard M :=
-  ⟨fun h => ⟨h.toIsMatching, fun T hT _ ↦ h.2 T hT⟩,
-    fun h => ⟨h.1, fun T hT ↦ (le_total T.encard M.encard).elim id <| h.2 hT⟩⟩
+lemma IsMatching.isMaxMatching_of_vertex_subset (hM : G.IsMatching M) (hsu : V(G) ⊆ V(G, M)) :
+    G.IsMaxMatching M where
+  toIsMatching := hM
+  max M' hM' := by
+    -- TODO: how to prove this easily?
 
-lemma matchingNumber_mono (hle : G ≤ H) : ν(G) ≤ ν(H) := by
-  sorry
+    -- sps |M| < |M'|, for contra
+    -- then there must be some e ∈ M' \ M
 
-
+    by_contra! hlt
+    -- TODO: i think this lemma is in the wrong file lol
+    have ⟨x, hx⟩ := diff_nonempty_of_encard_lt_encard hlt
+    sorry
 
 /-! ### Augmenting paths -/
 
-@[mk_iff]
-structure IsAltPath (G : Graph α β) (hM : G.IsMatching M) (P : WList α β) : Prop
-  extends G.IsPath P where
-  mem_matching : P.edge.IsChain (fun e f ↦ e ∈ M ∨ f ∈ M)
+noncomputable def IsPathGraph.first {P : Graph α β} (hP : P.IsPathGraph) : α :=
+  hP.choose.first
+
+noncomputable def IsPathGraph.last {P : Graph α β} (hP : P.IsPathGraph) : α :=
+  hP.choose.last
+
+-- probably want some generic "external/internal vxs/edges" for forests
+-- external vxs are just leaves
+-- internal vxs are non-leaves
+-- external edges are edges for which at least one endpoint is a leaf
+-- internal edges are edges for which both endpoints are not leaves
 
 @[mk_iff]
-structure IsSemiAugPath (G : Graph α β) (hM : G.IsMatching M) (P : WList α β) : Prop
-  extends G.IsAltPath hM P where
-  nonempty : P.Nonempty
-  last_not_in : P.last ∉ V(G, M)
-
-@[mk_iff]
-structure IsAugPath (G : Graph α β) (hM : G.IsMatching M) (P : WList α β) : Prop
-  extends G.IsSemiAugPath hM P where
-  first_not_in : P.first ∉ V(G, M)
+structure IsAugPath (G : Graph α β) (hM : G.IsMatching M) (P : Graph α β) : Prop where
+  subgraph : P ≤ G
+  isPathGraph : P.IsPathGraph
+  -- all internal vx of P are matched by M
+  -- matches_internal : M ∩ E(P) = E(P) \ {P.firstEdge, P.lastEdg e}
 
 /-! ### Structure of graph from maximal matching -/
 
@@ -144,17 +674,3 @@ structure IsOddCompOf (H G : Graph α β) extends H.IsCompOf G where
 
 def oddComponents (G : Graph α β) : Set (Graph α β) :=
   {H | H.IsOddCompOf G}
-
-/-! ### Cover -/
-
-structure IsCover (G : Graph α β) (S : Set α) : Prop where
-  subset : S ⊆ V(G)
-  cover : E(G) ⊆ E(G, S)
-
-structure IsMinCover (G : Graph α β) (S : Set α) : Prop extends IsCover G S where
-  min : ∀ T, IsCover G T → S.encard ≤ T.encard
-
-noncomputable def coverNumber (G : Graph α β) : ℕ∞ :=
-  sInf {n | ∃ S, G.IsCover S ∧ n = S.encard}
-
-scoped notation "τ(" G ")" => coverNumber G
